Parameterize language specification.

LinkerSpecification.v
@@ -7,9 +7,6 @@ Require Import Errors Behaviors Compiler Smallstep.
 
 Set Implicit Arguments.
 
-
-(* extended external function for C and Clight *)
-
 Definition external_function_ext :=
   (external_function * Ctypes.typelist * Ctypes.type * calling_convention)%type.
 
@@ -33,50 +30,151 @@ Proof.
   { apply external_function_eq. }
 Defined.
 
+(** Structures *)
 
-(* classify function definitions into internal and external functions  *)
+Structure Sig: Type := mkSig {
+  Sig_carrier :> Type;
+  Sig_dec: forall (sig1 sig2:Sig_carrier), {sig1 = sig2} + {sig1 <> sig2}
+}.
 
-Definition fundef_decT T F := T -> F + external_function.
+Structure F (sigT:Sig): Type := mkF {
+  F_carrier :> Type;
+  F_sig: forall (f:F_carrier), sigT
+}.
 
-Definition C_fundef_dec : fundef_decT Csyntax.fundef Csyntax.function :=
-  fun fundef =>
-    match fundef with
-      | Csyntax.Internal i => inl i
-      | Csyntax.External ef args res cc => inr ef
-    end.
+Structure EF (sigT:Sig): Type := mkEF {
+  EF_carrier :> Type;
+  EF_dec: forall (ef1 ef2:EF_carrier), {ef1 = ef2} + {ef1 <> ef2};
+  EF_linkable: forall (ef:EF_carrier), bool;
+  EF_sig: forall (ef:EF_carrier), sigT
+}.
 
-Definition Clight_fundef_dec : fundef_decT Clight.fundef Clight.function :=
-  fun fundef =>
-    match fundef with
-      | Clight.Internal i => inl i
-      | Clight.External ef args res cc => inr ef
-    end.
+Structure Fundef (sigT:Sig) (fT:F sigT) (efT:EF sigT) := mkFundef {
+  Fundef_carrier :> Type;
+  Fundef_dec: forall (fd:Fundef_carrier), fT + efT;
+  Fundef_sig :=
+    fun fd =>
+      match Fundef_dec fd with
+        | inl f => fT.(F_sig) f
+        | inr ef => efT.(EF_sig) ef
+      end
+}.
 
-Definition common_fundef_dec (F:Type) : fundef_decT (AST.fundef F) F :=
-  fun fundef =>
-    match fundef with
-      | Internal i => inl i
-      | External ef => inr ef
-    end.
+Structure V: Type := mkV {
+  V_carrier :> Type;
+  V_dec: forall (v1 v2:V_carrier), {v1 = v2} + {v1 <> v2}
+}.
 
+Structure Language: Type := mkLanguage {
+  sigT: Sig;
+  fT: F sigT;
+  efT: EF sigT;
+  fundefT: Fundef fT efT;
+  vT: V;
+
+  globdefT := AST.globdef fundefT vT;
+  progT := AST.program fundefT vT
+}.
+
+(** Canonical Structures *)
+
+Canonical Structure Sig_type: Sig := mkSig Ctypes.type_eq.
+Canonical Structure Sig_signature: Sig := mkSig signature_eq.
+
+Canonical Structure F_C: F Sig_type := mkF Sig_type Csyntax.type_of_function.
+Canonical Structure F_Clight: F Sig_type := mkF Sig_type Clight.type_of_function.
+Canonical Structure F_Csharpminor: F Sig_signature := mkF Sig_signature Csharpminor.fn_sig.
+Canonical Structure F_Cminor: F Sig_signature := mkF Sig_signature Cminor.fn_sig.
+Canonical Structure F_CminorSel: F Sig_signature := mkF Sig_signature CminorSel.fn_sig.
+Canonical Structure F_RTL: F Sig_signature := mkF Sig_signature RTL.fn_sig.
+Canonical Structure F_LTL: F Sig_signature := mkF Sig_signature LTL.fn_sig.
+Canonical Structure F_Linear: F Sig_signature := mkF Sig_signature Linear.fn_sig.
+Canonical Structure F_Mach: F Sig_signature := mkF Sig_signature Mach.fn_sig.
+Canonical Structure F_Asm: F Sig_signature := mkF Sig_signature Asm.fn_sig.
+
+Canonical Structure EF_external_function_ext: EF Sig_type :=
+  mkEF Sig_type
+       external_function_ext_eq
+       (fun ef => match ef with (EF_external _ _, _, _, _) => true | _ => false end)
+       (fun ef => match ef with (_, targs, tres, cc) => Ctypes.Tfunction targs tres cc end).
+Canonical Structure EF_external_function: EF Sig_signature :=
+  mkEF Sig_signature
+       external_function_eq
+       (fun ef => match ef with EF_external _ _ => true | _ => false end)
+       ef_sig.
+
+Canonical Structure Fundef_C: Fundef F_C EF_external_function_ext :=
+  mkFundef F_C EF_external_function_ext
+           (fun fd =>
+              match fd with
+                | Csyntax.Internal f => inl f
+                | Csyntax.External ef targs tres cc => inr (ef, targs, tres, cc)
+              end).
+Canonical Structure Fundef_Clight: Fundef F_Clight EF_external_function_ext :=
+  mkFundef F_Clight EF_external_function_ext
+           (fun fd =>
+              match fd with
+                | Clight.Internal f => inl f
+                | Clight.External ef targs tres cc => inr (ef, targs, tres, cc)
+              end).
+Canonical Structure Fundef_common (fT:F Sig_signature): Fundef fT EF_external_function :=
+  mkFundef fT EF_external_function
+           (fun fd =>
+              match fd with
+                | AST.Internal f => inl f
+                | AST.External ef => inr ef
+              end).
+
+Canonical Structure V_type: V := mkV Ctypes.type_eq.
+Canonical Structure V_unit: V := mkV unit_eq.
+
+Canonical Structure Language_C: Language := mkLanguage Fundef_C V_type.
+Canonical Structure Language_Clight: Language := mkLanguage Fundef_Clight V_type.
+Canonical Structure Language_Csharpminor: Language := mkLanguage (Fundef_common F_Csharpminor) V_unit.
+Canonical Structure Language_Cminor: Language := mkLanguage (Fundef_common F_Cminor) V_unit.
+Canonical Structure Language_CminorSel: Language := mkLanguage (Fundef_common F_CminorSel) V_unit.
+Canonical Structure Language_RTL: Language := mkLanguage (Fundef_common F_RTL) V_unit.
+Canonical Structure Language_LTL: Language := mkLanguage (Fundef_common F_LTL) V_unit.
+Canonical Structure Language_Linear: Language := mkLanguage (Fundef_common F_Linear) V_unit.
+Canonical Structure Language_Mach: Language := mkLanguage (Fundef_common F_Mach) V_unit.
+Canonical Structure Language_Asm: Language := mkLanguage (Fundef_common F_Asm) V_unit.
 
 (** Linker definition *)
 Section LINKER.
 
-Variable (fundefT F V:Type).
-Variable (fundef_dec: fundef_decT fundefT F).
-Variable (V_dec: forall (v1 v2:V), {v1 = v2} + {v1 <> v2}).
+Variable (lang:Language).
+  
+Let sigT := lang.(sigT).
+Let fT := lang.(fT).
+Let efT := lang.(efT).
+Let fundefT := lang.(fundefT).
+Let vT := lang.(vT).
+
+Let f_sig := fT.(F_sig).
+Let ef_sig := efT.(EF_sig).
+Let ef_dec := efT.(EF_dec).
+Let fundef_dec := fundefT.(Fundef_dec).
+Let v_dec := vT.(V_dec).
+
+Ltac clarify :=
+  repeat
+    (try match goal with
+           | [H1: fundef_dec ?f = _, H2: fundef_dec ?f = _ |- _] =>
+             rewrite H1 in H2; inv H2
+         end;
+     auto).
 
 (** `linkable a b` means we can remove `a` and take `b` when the two are linked. *)
 
 Inductive globfun_linkable (f1 f2:fundefT): Prop :=
 | globfun_linkable_ei (* TODO: type check? *)
     e1 i2 (H1: fundef_dec f1 = inr e1) (H2: fundef_dec f2 = inl i2)
+    (Hsig: ef_sig e1 = f_sig i2)
 | globfun_linkable_ee
     e (H1: fundef_dec f1 = inr e) (H1: fundef_dec f2 = inr e)
 .
 
-Inductive globvar_linkable (v1 v2:globvar V): Prop :=
+Inductive globvar_linkable (v1 v2:globvar vT): Prop :=
 | globvar_linkable_intro
     (Hinfo: v1.(gvar_info) = v2.(gvar_info))
     (Hinit: v1.(gvar_init) = nil)
@@ -84,7 +182,7 @@ Inductive globvar_linkable (v1 v2:globvar V): Prop :=
     (Hvolatile: v1.(gvar_volatile) = v2.(gvar_volatile))
 .
 
-Inductive globdef_linkable: forall (g1 g2:globdef fundefT V), Prop :=
+Inductive globdef_linkable: forall (g1 g2:globdef fundefT vT), Prop :=
 | globdef_linkable_fun
     f1 f2 (Hv: globfun_linkable f1 f2):
     globdef_linkable (Gfun f1) (Gfun f2)
@@ -104,16 +202,12 @@ Proof.
     - rewrite Hf1 in H1. inv H1.
   }
   destruct (fundef_dec f2) as [i2|e2] eqn:Hf2.
-  { left. econstructor; eauto. }
-  { destruct (external_function_eq e1 e2); [subst|].
-    { left. eapply globfun_linkable_ee; eauto. }
-    { right. contradict n. inv n; auto.
-      - rewrite Hf2 in H2. inv H2.
-      - rewrite Hf1 in H1. inv H1.
-        rewrite Hf2 in H0. inv H0.
-        auto.
-    }
-  }
+  - destruct (sigT.(Sig_dec) (ef_sig e1) (f_sig i2)).
+    + left. econstructor; eauto.
+    + right. contradict n. inv n; clarify.
+  - destruct (ef_dec e1 e2); [subst|].
+    + left. eapply globfun_linkable_ee; eauto.
+    + right. contradict n. inv n; clarify.
 Defined.
 
 Definition init_data_dec (v1 v2:init_data): {v1 = v2} + {v1 <> v2}.
@@ -127,13 +221,13 @@ Proof.
   (try apply ident_eq).
 Defined.
 
-Definition globvar_linkable_dec (v1 v2:globvar V): {globvar_linkable v1 v2} + {~ globvar_linkable v1 v2}.
+Definition globvar_linkable_dec (v1 v2:globvar vT): {globvar_linkable v1 v2} + {~ globvar_linkable v1 v2}.
 Proof.
   destruct v1 as [info1 init1 readonly1 volatile1].
   destruct v2 as [info2 init2 readonly2 volatile2].
   destruct (bool_dec readonly1 readonly2); [subst|].
   { destruct (bool_dec volatile1 volatile2); [subst|].
-    { destruct (V_dec info1 info2); [subst|].
+    { destruct (v_dec info1 info2); [subst|].
       { destruct (list_eq_dec init_data_dec init1 nil).
         { left. constructor; simpl in *; auto. }
         { right. intro X. inv X. simpl in *.
@@ -141,7 +235,7 @@ Proof.
         }
       }
       { right. contradict n. inv n. simpl in *.
-        destruct (V_dec info1 info2); auto.
+        destruct (v_dec info1 info2); auto.
       }
     }
     { right. contradict n. inv n. auto. }
@@ -149,7 +243,7 @@ Proof.
   { right. contradict n. inv n. auto. }
 Defined.
 
-Definition globdef_linkable_dec (g1 g2:globdef fundefT V): {globdef_linkable g1 g2} + {~ globdef_linkable g1 g2}.
+Definition globdef_linkable_dec (g1 g2:globdef fundefT vT): {globdef_linkable g1 g2} + {~ globdef_linkable g1 g2}.
 Proof.
   destruct g1 as [f1|v1], g2 as [f2|v2].
   { destruct (globfun_linkable_dec f1 f2).
@@ -167,7 +261,7 @@ Defined.
 
 (** main definition *)
 
-Definition link_globdefs (defs1 defs2:PTree.t (globdef fundefT V)): option (PTree.t (globdef fundefT V)) :=
+Definition link_globdefs (defs1 defs2:PTree.t (globdef fundefT vT)): option (PTree.t (globdef fundefT vT)) :=
   let defs :=
     PTree.combine
       (fun odef1 odef2 =>
@@ -194,13 +288,13 @@ Definition link_globdefs (defs1 defs2:PTree.t (globdef fundefT V)): option (PTre
   then Some (PTree_option_map (fun _ x => x) defs)
   else None.
 
-Definition link_globdef_list (defs1 defs2:list (positive * globdef fundefT V)): option (list (positive * globdef fundefT V)) :=
+Definition link_globdef_list (defs1 defs2:list (positive * globdef fundefT vT)): option (list (positive * globdef fundefT vT)) :=
   match link_globdefs (PTree_unelements defs1) (PTree_unelements defs2) with
     | Some defs => Some (PTree.elements defs)
     | None => None
   end.
 
-Definition link_program (prog1 prog2:program fundefT V): option (program fundefT V) :=
+Definition link_program (prog1 prog2:program fundefT vT): option (program fundefT vT) :=
   match
     Pos.eqb prog1.(prog_main) prog2.(prog_main),
     link_globdef_list prog1.(prog_defs) prog2.(prog_defs)
@@ -219,8 +313,8 @@ Inductive separately_compiled: forall (cprog: Csyntax.program) (asmprog: Asm.pro
 | separately_compiled_link cprog1 cprog2 asmprog1 asmprog2
           (H1: separately_compiled cprog1 asmprog1)
           (H2: separately_compiled cprog2 asmprog2)
-          cprog (Hcprog: Some cprog = link_program C_fundef_dec Ctypes.type_eq cprog1 cprog2)
-          asmprog (Hasmprog: Some asmprog = link_program (@common_fundef_dec Asm.function) unit_eq asmprog1 asmprog2):
+          cprog (Hcprog: Some cprog = link_program Language_C cprog1 cprog2)
+          asmprog (Hasmprog: Some asmprog = link_program Language_Asm asmprog1 asmprog2):
     separately_compiled cprog asmprog
 .
 
