common/ProgramLSim.v
@@ -19,66 +19,94 @@ Qed.
 (* lifting function simulation to program simulation *)
 Section PROGRAM_LSIM.
 
-Variable (fundefT_src F_src V_src:Type).
-Variable (fundef_src_dec: fundef_decT fundefT_src F_src).
-Variable (V_src_dec: forall (v1 v2:V_src), {v1 = v2} + {v1 <> v2}).
-Variable (F_sig_src: forall (f:F_src), signature).
-Let fundef_sig_src (fundef:fundefT_src): signature :=
-  match fundef_src_dec fundef with
-    | inl f => F_sig_src f
-    | inr ef => ef_sig ef
-  end.
+Variable (lang_src lang_tgt:Language).
+  
+Let sigT_src := lang_src.(sigT).
+Let fT_src := lang_src.(fT).
+Let efT_src := lang_src.(efT).
+Let fundefT_src := lang_src.(fundefT).
+Let vT_src := lang_src.(vT).
 
-Variable (fundefT_tgt F_tgt V_tgt:Type).
-Variable (fundef_tgt_dec: fundef_decT fundefT_tgt F_tgt).
-Variable (V_tgt_dec: forall (v1 v2:V_tgt), {v1 = v2} + {v1 <> v2}).
-Variable (F_sig_tgt: forall (f:F_tgt), signature).
-Let fundef_sig_tgt (fundef:fundefT_tgt): signature :=
-  match fundef_tgt_dec fundef with
-    | inl f => F_sig_tgt f
-    | inr ef => ef_sig ef
-  end.
+Let f_sig_src := fT_src.(F_sig).
+Let ef_sig_src := efT_src.(EF_sig).
+Let fd_sig_src := fundefT_src.(Fundef_sig).
+Let ef_dec_src := efT_src.(EF_dec).
+Let fundef_dec_src := fundefT_src.(Fundef_dec).
+Let v_dec_src := vT_src.(V_dec).
 
-Variable (transf_V: forall (v:V_src), res V_tgt).
-Let V_lsim (v_src:V_src) (v_tgt:V_tgt) := transf_V v_src = OK v_tgt.
+Let sigT_tgt := lang_tgt.(sigT).
+Let fT_tgt := lang_tgt.(fT).
+Let efT_tgt := lang_tgt.(efT).
+Let fundefT_tgt := lang_tgt.(fundefT).
+Let vT_tgt := lang_tgt.(vT).
 
-Definition F_lsimT :=
+Let f_sig_tgt := fT_tgt.(F_sig).
+Let ef_sig_tgt := efT_tgt.(EF_sig).
+Let fd_sig_tgt := fundefT_tgt.(Fundef_sig).
+Let ef_dec_tgt := efT_tgt.(EF_dec).
+Let fundef_dec_tgt := fundefT_tgt.(Fundef_dec).
+Let v_dec_tgt := vT_tgt.(V_dec).
+
+Variable (transf_sigT: forall (ef:sigT_src), sigT_tgt).
+Variable (transf_efT: forall (ef:efT_src), res efT_tgt).
+Variable (transf_vT: forall (v:vT_src), res vT_tgt).
+Hypothesis transf_efT_sigT: forall ef_src ef_tgt (H: transf_efT ef_src = OK ef_tgt), transf_sigT (ef_sig_src ef_src) = ef_sig_tgt ef_tgt.
+
+Let sig_lsim (sig_src:sigT_src) (sig_tgt:sigT_tgt) := transf_sigT sig_src = sig_tgt.
+Let ef_lsim (ef_src:efT_src) (ef_tgt:efT_tgt) := transf_efT ef_src = OK ef_tgt.
+Let v_lsim (v_src:vT_src) (v_tgt:vT_tgt) := transf_vT v_src = OK v_tgt.
+
+Definition f_lsimT :=
   forall
-    (fprog_src:program fundefT_src V_src)
-    (fprog_tgt:program fundefT_tgt V_tgt)
-    (f_src:F_src) (f_tgt:F_tgt), Prop.
+    (fprog_src:lang_src.(progT)) (fprog_tgt:lang_tgt.(progT))
+    (f_src:fT_src) (f_tgt:fT_tgt), Prop.
+
+Ltac clarify :=
+  unfold fd_sig_src, fd_sig_tgt, Fundef_sig, f_sig_src, f_sig_tgt, ef_sig_src, ef_sig_tgt in *;
+  unfold fundefT_src, vT_src, fundefT_tgt, vT_tgt, fundef_dec_src, fundef_dec_tgt in *;
+  unfold fT_src, fT_tgt, efT_src, efT_tgt in *;
+  repeat
+    (try match goal with
+           | [H1: Fundef_dec ?fundefT ?f = _, H2: Fundef_dec ?fundefT ?f = _ |- _] =>
+             rewrite H1 in H2; inv H2
+           | [H: match ?x with | inl _ => False | inr _ => _ end |- _] =>
+             let Hx := fresh "Hx" in destruct x eqn:Hx; [inv H|]
+           | [H: match ?x with | inr _ => False | inl _ => _ end |- _] =>
+             let Hx := fresh "Hx" in destruct x eqn:Hx; [|inv H]
+           | [H: False |- _] => inv H
+         end;
+     auto).
 
 Section CORE.
 
-Variable (F_lsim:F_lsimT).
-Variable (prog_src:program fundefT_src V_src).
-Variable (prog_tgt:program fundefT_tgt V_tgt).
+Variable (f_lsim:f_lsimT).
+Variable (prog_src:lang_src.(progT)).
+Variable (prog_tgt:lang_tgt.(progT)).
 
-Inductive globvar_lsim (v_src:globvar V_src) (v_tgt:globvar V_tgt): Prop :=
+Inductive globvar_lsim (v_src:globvar vT_src) (v_tgt:globvar vT_tgt): Prop :=
 | globvar_lsim_intro
-    (Hv: transf_globvar transf_V v_src = OK v_tgt)
+    (Hv: transf_globvar transf_vT v_src = OK v_tgt)
 .
 
 (** simulation *)
 Inductive globfun_lsim
           (g_src:fundefT_src) (g_tgt:fundefT_tgt): Prop :=
-| globfun_lsim_i
-    f_src f_tgt
-    (Hsrc: fundef_src_dec g_src = inl f_src)
-    (Htgt: fundef_tgt_dec g_tgt = inl f_tgt)
-    (Hsim: forall fprog_src fprog_tgt
-                  (Hfprog_src: program_linkeq fundef_src_dec prog_src fprog_src)
-                  (Hfprog_tgt: program_linkeq fundef_tgt_dec prog_tgt fprog_tgt),
-             F_lsim fprog_src fprog_tgt f_src f_tgt /\
-             F_sig_src f_src = F_sig_tgt f_tgt)
-| globfun_lsim_e
-    ef
-    (Hsrc: fundef_src_dec g_src = inr ef)
-    (Htgt: fundef_tgt_dec g_tgt = inr ef)
-.
+| globfun_lsim_intro
+    (Hsim:
+       match fundef_dec_src g_src, fundef_dec_tgt g_tgt with
+         | inl f_src, inl f_tgt =>
+           forall fprog_src fprog_tgt
+                  (Hfprog_src: program_linkeq lang_src prog_src fprog_src)
+                  (Hfprog_tgt: program_linkeq lang_tgt prog_tgt fprog_tgt),
+             f_lsim fprog_src fprog_tgt f_src f_tgt /\
+             sig_lsim (f_sig_src f_src) (f_sig_tgt f_tgt)
+         | inr ef_src, inr ef_tgt =>
+           ef_lsim ef_src ef_tgt
+         | _, _ => False
+       end).
 
 Inductive globdef_lsim:
-  forall (g_src:globdef fundefT_src V_src) (g_tgt:globdef fundefT_tgt V_tgt), Prop :=
+  forall (g_src:globdef fundefT_src vT_src) (g_tgt:globdef fundefT_tgt vT_tgt), Prop :=
 | globdef_lsim_fun
     f_src f_tgt (Hf: globfun_lsim f_src f_tgt):
     globdef_lsim (Gfun f_src) (Gfun f_tgt)
@@ -88,8 +116,8 @@ Inductive globdef_lsim:
 .
 
 Definition globdefs_lsim
-           (defs_src:PTree.t (globdef fundefT_src V_src))
-           (defs_tgt:PTree.t (globdef fundefT_tgt V_tgt)): Prop :=
+           (defs_src:PTree.t (globdef fundefT_src vT_src))
+           (defs_tgt:PTree.t (globdef fundefT_tgt vT_tgt)): Prop :=
   forall i,
     match PTree.get i defs_src, PTree.get i defs_tgt with
       | Some g1, Some g2 => globdef_lsim g1 g2
@@ -98,8 +126,8 @@ Definition globdefs_lsim
     end.
 
 Definition globdef_list_lsim
-           (defs_src:list (positive * globdef fundefT_src V_src))
-           (defs_tgt:list (positive * globdef fundefT_tgt V_tgt)): Prop :=
+           (defs_src:list (positive * globdef fundefT_src vT_src))
+           (defs_tgt:list (positive * globdef fundefT_tgt vT_tgt)): Prop :=
   list_forall2
     (fun g_src g_tgt =>
        fst g_src = fst g_tgt /\
@@ -115,33 +143,32 @@ End CORE.
 (** an instantiation of weak simulation: matching any function definitions *)
 Definition program_weak_lsim := program_lsim_aux (fun _ _ _ _ => True).
 
-(** properties on F_lsim and simulation *)
+(** properties on f_lsim and simulation *)
 Lemma globfun_lsim_le
-      (F_lsim1 F_lsim2:F_lsimT)
-      (prog1_src prog2_src:program fundefT_src V_src)
-      (prog1_tgt prog2_tgt:program fundefT_tgt V_tgt)
-      (HF_lsim: F_lsim1 <4= F_lsim2)
-      (Hprog_src: program_linkeq fundef_src_dec prog1_src prog2_src)
-      (Hprog_tgt: program_linkeq fundef_tgt_dec prog1_tgt prog2_tgt):
-  (globfun_lsim F_lsim1 prog1_src prog1_tgt) <2= (globfun_lsim F_lsim2 prog2_src prog2_tgt).
+      (f_lsim1 f_lsim2:f_lsimT)
+      (prog1_src prog2_src:program fundefT_src vT_src)
+      (prog1_tgt prog2_tgt:program fundefT_tgt vT_tgt)
+      (Hf_lsim: f_lsim1 <4= f_lsim2)
+      (Hprog_src: program_linkeq lang_src prog1_src prog2_src)
+      (Hprog_tgt: program_linkeq lang_tgt prog1_tgt prog2_tgt):
+  (globfun_lsim f_lsim1 prog1_src prog1_tgt) <2= (globfun_lsim f_lsim2 prog2_src prog2_tgt).
 Proof.
-  intros. inv PR.
-  - eapply globfun_lsim_i; eauto.
-    intros. exploit Hsim; eauto. intros [Hsim1 Hsig].
-    split; auto. apply HF_lsim. eapply Hsim.
-    + rewrite Hprog_src. auto.
-    + rewrite Hprog_tgt. auto.
-  - eapply globfun_lsim_e; eauto.
+  intros. inv PR; constructor.
+  destruct (fundef_dec_src x0), (fundef_dec_tgt x1); auto.
+  intros. exploit Hsim; eauto. intros [Hsim1 Hsig].
+  split; auto. apply Hf_lsim. eapply Hsim.
+  + rewrite Hprog_src. auto.
+  + rewrite Hprog_tgt. auto.
 Qed.
 
 Lemma globdef_lsim_le
-      (F_lsim1 F_lsim2:F_lsimT)
-      (prog1_src prog2_src:program fundefT_src V_src)
-      (prog1_tgt prog2_tgt:program fundefT_tgt V_tgt)
-      (HF_lsim: F_lsim1 <4= F_lsim2)
-      (Hprog_src: program_linkeq fundef_src_dec prog1_src prog2_src)
-      (Hprog_tgt: program_linkeq fundef_tgt_dec prog1_tgt prog2_tgt):
-  (globdef_lsim F_lsim1 prog1_src prog1_tgt) <2= (globdef_lsim F_lsim2 prog2_src prog2_tgt).
+      (f_lsim1 f_lsim2:f_lsimT)
+      (prog1_src prog2_src:program fundefT_src vT_src)
+      (prog1_tgt prog2_tgt:program fundefT_tgt vT_tgt)
+      (Hf_lsim: f_lsim1 <4= f_lsim2)
+      (Hprog_src: program_linkeq lang_src prog1_src prog2_src)
+      (Hprog_tgt: program_linkeq lang_tgt prog1_tgt prog2_tgt):
+  (globdef_lsim f_lsim1 prog1_src prog1_tgt) <2= (globdef_lsim f_lsim2 prog2_src prog2_tgt).
 Proof.
   intros. inv PR.
   - eapply globdef_lsim_fun; eauto.
@@ -150,13 +177,13 @@ Proof.
 Qed.
 
 Lemma globdef_list_lsim_le
-      (F_lsim1 F_lsim2:F_lsimT)
-      (prog1_src prog2_src:program fundefT_src V_src)
-      (prog1_tgt prog2_tgt:program fundefT_tgt V_tgt)
-      (HF_lsim: F_lsim1 <4= F_lsim2)
-      (Hprog_src: program_linkeq fundef_src_dec prog1_src prog2_src)
-      (Hprog_tgt: program_linkeq fundef_tgt_dec prog1_tgt prog2_tgt):
-  (globdef_list_lsim F_lsim1 prog1_src prog1_tgt) <2= (globdef_list_lsim F_lsim2 prog2_src prog2_tgt).
+      (f_lsim1 f_lsim2:f_lsimT)
+      (prog1_src prog2_src:program fundefT_src vT_src)
+      (prog1_tgt prog2_tgt:program fundefT_tgt vT_tgt)
+      (Hf_lsim: f_lsim1 <4= f_lsim2)
+      (Hprog_src: program_linkeq lang_src prog1_src prog2_src)
+      (Hprog_tgt: program_linkeq lang_tgt prog1_tgt prog2_tgt):
+  (globdef_list_lsim f_lsim1 prog1_src prog1_tgt) <2= (globdef_list_lsim f_lsim2 prog2_src prog2_tgt).
 Proof.
   intros.
   eapply list_forall2_imply; eauto. simpl. intros.
@@ -165,9 +192,9 @@ Proof.
 Qed.
 
 Lemma program_lsim_aux_le
-      (F_lsim1 F_lsim2:F_lsimT)
-      (HF_lsim: F_lsim1 <4= F_lsim2):
-  (program_lsim_aux F_lsim1) <2= (program_lsim_aux F_lsim2).
+      (f_lsim1 f_lsim2:f_lsimT)
+      (Hf_lsim: f_lsim1 <4= f_lsim2):
+  (program_lsim_aux f_lsim1) <2= (program_lsim_aux f_lsim2).
 Proof.
   intros prog_src prog_tgt Hsim.
   destruct prog_src as [defs_src main_src].
@@ -181,13 +208,13 @@ Qed.
 (** globdefs_lsim and globdef_list_lsim *)
 
 Lemma globdefs_lsim_globdef_list_lsim
-      (F_lsim:F_lsimT)
-      (fprog_src:program fundefT_src V_src)
-      (fprog_tgt:program fundefT_tgt V_tgt)
-      (defs_src: PTree.t (globdef fundefT_src V_src))
-      (defs_tgt: PTree.t (globdef fundefT_tgt V_tgt))
-      (Hsim: globdefs_lsim F_lsim fprog_src fprog_tgt defs_src defs_tgt):
-  globdef_list_lsim F_lsim fprog_src fprog_tgt (PTree.elements defs_src) (PTree.elements defs_tgt).
+      (f_lsim:f_lsimT)
+      (fprog_src:program fundefT_src vT_src)
+      (fprog_tgt:program fundefT_tgt vT_tgt)
+      (defs_src: PTree.t (globdef fundefT_src vT_src))
+      (defs_tgt: PTree.t (globdef fundefT_tgt vT_tgt))
+      (Hsim: globdefs_lsim f_lsim fprog_src fprog_tgt defs_src defs_tgt):
+  globdef_list_lsim f_lsim fprog_src fprog_tgt (PTree.elements defs_src) (PTree.elements defs_tgt).
 Proof.
   apply PTree.elements_canonical_order; intros.
   - exploit Hsim. instantiate (1 := i). rewrite H. intro X.
@@ -199,13 +226,13 @@ Proof.
 Qed.
 
 Lemma globdef_list_lsim_globdefs_lsim
-      (F_lsim:F_lsimT)
-      (fprog_src:program fundefT_src V_src)
-      (fprog_tgt:program fundefT_tgt V_tgt)
-      (defs_src: list (positive * (globdef fundefT_src V_src)))
-      (defs_tgt: list (positive * (globdef fundefT_tgt V_tgt)))
-      (Hsim: globdef_list_lsim F_lsim fprog_src fprog_tgt defs_src defs_tgt):
-  globdefs_lsim F_lsim fprog_src fprog_tgt (PTree_unelements defs_src) (PTree_unelements defs_tgt).
+      (f_lsim:f_lsimT)
+      (fprog_src:program fundefT_src vT_src)
+      (fprog_tgt:program fundefT_tgt vT_tgt)
+      (defs_src: list (positive * (globdef fundefT_src vT_src)))
+      (defs_tgt: list (positive * (globdef fundefT_tgt vT_tgt)))
+      (Hsim: globdef_list_lsim f_lsim fprog_src fprog_tgt defs_src defs_tgt):
+  globdefs_lsim f_lsim fprog_src fprog_tgt (PTree_unelements defs_src) (PTree_unelements defs_tgt).
 Proof.
   unfold globdefs_lsim, globdef_list_lsim in *. intro i.
   rewrite ? PTree_guespec. apply list_forall2_rev in Hsim.
@@ -217,53 +244,43 @@ Proof.
 Qed.
 
 (** properties of linking on simulation *)
-Ltac simplify_decs :=
-  repeat
-    match goal with
-      | [Hl: fundef_src_dec ?f = _,
-         Hr: fundef_src_dec ?f = _ |- _] =>
-        rewrite Hl in Hr; inv Hr
-      | [Hl: fundef_tgt_dec ?f = _,
-         Hr: fundef_tgt_dec ?f = _ |- _] =>
-        rewrite Hl in Hr; inv Hr
-    end.
 
 Lemma link_globdefs_lsim
-      (F_lsim:F_lsimT)
+      (f_lsim:f_lsimT)
       (main:positive)
-      (defs1_src defs2_src:list (positive * globdef fundefT_src V_src))
-      (defs1_tgt defs2_tgt:list (positive * globdef fundefT_tgt V_tgt))
-      defs_src (Hdefs_src: link_globdefs fundef_src_dec V_src_dec (PTree_unelements defs1_src) (PTree_unelements defs2_src) = Some defs_src)
+      (defs1_src defs2_src:list (positive * globdef fundefT_src vT_src))
+      (defs1_tgt defs2_tgt:list (positive * globdef fundefT_tgt vT_tgt))
+      defs_src (Hdefs_src: link_globdefs lang_src (PTree_unelements defs1_src) (PTree_unelements defs2_src) = Some defs_src)
       (H1: globdefs_lsim
-             F_lsim
+             f_lsim
              (mkprogram defs1_src main)
              (mkprogram defs1_tgt main)
              (PTree_unelements defs1_src)
              (PTree_unelements defs1_tgt))
       (H2: globdefs_lsim
-             F_lsim
+             f_lsim
              (mkprogram defs2_src main)
              (mkprogram defs2_tgt main)
              (PTree_unelements defs2_src)
              (PTree_unelements defs2_tgt)):
   exists defs_tgt,
-    link_globdefs fundef_tgt_dec V_tgt_dec (PTree_unelements defs1_tgt) (PTree_unelements defs2_tgt) = Some defs_tgt /\
+    link_globdefs lang_tgt (PTree_unelements defs1_tgt) (PTree_unelements defs2_tgt) = Some defs_tgt /\
     globdefs_lsim
-      F_lsim
+      f_lsim
       (mkprogram (PTree.elements defs_src) main)
       (mkprogram (PTree.elements defs_tgt) main)
       defs_src defs_tgt.
 Proof.
-  generalize (link_globdefs_linkeq_l _ _ _ _ Hdefs_src). intro Hle1_src.
-  generalize (link_globdefs_linkeq_r _ _ _ _ Hdefs_src). intro Hle2_src.
-  destruct (link_globdefs fundef_tgt_dec V_tgt_dec (PTree_unelements defs1_tgt) (PTree_unelements defs2_tgt)) as [defs_tgt|] eqn:Hdefs_tgt.
-  { generalize (link_globdefs_linkeq_l _ _ _ _ Hdefs_tgt). intro Hle1_tgt.
-    generalize (link_globdefs_linkeq_r _ _ _ _ Hdefs_tgt). intro Hle2_tgt.
+  generalize (link_globdefs_linkeq_l _ _ _ Hdefs_src). intro Hle1_src.
+  generalize (link_globdefs_linkeq_r _ _ _ Hdefs_src). intro Hle2_src.
+  destruct (link_globdefs lang_tgt (PTree_unelements defs1_tgt) (PTree_unelements defs2_tgt)) as [defs_tgt|] eqn:Hdefs_tgt.
+  { generalize (link_globdefs_linkeq_l _ _ _ Hdefs_tgt). intro Hle1_tgt.
+    generalize (link_globdefs_linkeq_r _ _ _ Hdefs_tgt). intro Hle2_tgt.
     eexists. split; [eauto|].
     intro i. 
     eapply gtlink_globdefs in Hdefs_src. instantiate (1 := i) in Hdefs_src.
     eapply gtlink_globdefs in Hdefs_tgt. instantiate (1 := i) in Hdefs_tgt.
-    specialize (H1 i). specialize (H2 i).
+    specialize (H1 i). specialize (H2 i). clarify.
     destruct ((PTree_unelements defs1_src) ! i) eqn:Hi1_src,
              ((PTree_unelements defs2_src) ! i) eqn:Hi2_src,
              (defs_src ! i) eqn:Hi_src; subst; try (inv Hdefs_src; fail);
@@ -271,15 +288,7 @@ Proof.
              ((PTree_unelements defs2_tgt) ! i) eqn:Hi2_tgt,
              (defs_tgt ! i) eqn:Hi_tgt; subst; try (inv Hdefs_tgt; fail);
     try (inv H1; fail); try (inv H2; fail); auto.
-    { destruct Hdefs_src as [[]|[]], Hdefs_tgt as [[]|[]]; subst;
-      repeat
-        match goal with
-          | [H: globfun_lsim _ _ _ _ _ |- _] => inv H
-          | [H1: fundef_src_dec ?f = _, H2: fundef_src_dec ?f = _ |- _] =>
-            rewrite H1 in H2; inv H2
-          | [H1: fundef_tgt_dec ?f = _, H2: fundef_tgt_dec ?f = _ |- _] =>
-            rewrite H1 in H2; inv H2
-        end.
+    { destruct Hdefs_src as [[]|[]], Hdefs_tgt as [[]|[]]; subst; clarify.
       - eapply globdef_lsim_le; eauto.
         + split; auto. unfold globdef_list_linkeq. rewrite Hle2_src.
           repeat intro. exists def1. split; [|reflexivity].
@@ -287,59 +296,28 @@ Proof.
         + split; auto. unfold globdef_list_linkeq. rewrite Hle2_tgt.
           repeat intro. exists def1. split; [|reflexivity].
           simpl. rewrite PTree_unelements_elements. auto.
-      - inv H; inv H1; inv H2; inv H3; inv Hv; inv Hv0; repeat constructor;
-        repeat
-          match goal with
-            | [H: globfun_lsim _ _ _ _ _ |- _] => inv H
-            | [H1: fundef_src_dec ?f = _, H2: fundef_src_dec ?f = _ |- _] =>
-              rewrite H1 in H2; inv H2
-            | [H1: fundef_tgt_dec ?f = _, H2: fundef_tgt_dec ?f = _ |- _] =>
-              rewrite H1 in H2; inv H2
-          end.
-        + eapply globfun_lsim_e; eauto.
-        + inv Hv1. destruct v1, v2; simpl in *; subst.
-          unfold transf_globvar in *. simpl in *.
-          destruct (transf_V gvar_info0); simpl in *; inv Hv; inv Hv0.
-          inv Hv2. simpl in *. subst. auto.
-      - inv H; inv H1; inv H2; inv H3; inv Hv; inv Hv0; repeat constructor;
-        repeat
-          match goal with
-            | [H: globfun_lsim _ _ _ _ _ |- _] => inv H
-            | [H1: fundef_src_dec ?f = _, H2: fundef_src_dec ?f = _ |- _] =>
-              rewrite H1 in H2; inv H2
-            | [H1: fundef_tgt_dec ?f = _, H2: fundef_tgt_dec ?f = _ |- _] =>
-              rewrite H1 in H2; inv H2
-          end.
-        + eapply globfun_lsim_e; eauto.
-        + inv Hv1. destruct v1, v2; simpl in *; subst.
-          unfold transf_globvar in *. simpl in *.
-          destruct (transf_V gvar_info0); simpl in *; inv Hv; inv Hv0.
-          inv Hv2. simpl in *. subst. auto.
-      - inv H; inv H1; inv H2; inv H3; inv Hv; inv Hv0; repeat constructor;
-        repeat
-          match goal with
-            | [H: globfun_lsim _ _ _ _ _ |- _] => inv H
-            | [H1: fundef_src_dec ?f = _, H2: fundef_src_dec ?f = _ |- _] =>
-              rewrite H1 in H2; inv H2
-            | [H1: fundef_tgt_dec ?f = _, H2: fundef_tgt_dec ?f = _ |- _] =>
-              rewrite H1 in H2; inv H2
-          end.
-        + eapply globfun_lsim_i; eauto. intros. apply Hsim.
-          * destruct Hfprog_src as [Hfdefs_src ?]. simpl in *. subst.
-            split; auto. unfold globdef_list_linkeq in *.
-            rewrite Hle1_src, <- Hfdefs_src.
-            repeat intro. exists def1. split; [|reflexivity].
-            rewrite PTree_unelements_elements. auto.
-          * destruct Hfprog_tgt as [Hfdefs_tgt ?]. simpl in *. subst.
-            split; auto. unfold globdef_list_linkeq in *.
-            rewrite Hle1_tgt, <- Hfdefs_tgt.
-            repeat intro. exists def1. split; [|reflexivity].
-            rewrite PTree_unelements_elements. auto.
-        + eapply globfun_lsim_e; eauto.
-        + inv Hv1. destruct v1, v2; simpl in *; subst.
-          unfold transf_globvar in *. simpl in *.
-          destruct (transf_V gvar_info0); simpl in *; inv Hv; inv Hv0.
-          inv Hv2. simpl in *. subst. auto.
+      - inv H; inv H1; inv H2; inv H3; inv Hv; inv Hv0; try inv Hf; try inv Hf0; clarify;
+        repeat constructor; clarify;
+        rewrite ? H1, ? H2, ? H0, ? H3 in *; clarify.
+        inv Hv1. inv Hv2. unfold transf_globvar in *. rewrite Hinfo in *.
+        clarify. destruct (transf_vT (gvar_info v2)); inv Hv; inv Hv0.
+        simpl in *. f_equal. f_equal; auto. rewrite Hinit, Hinit0. auto.
+      - inv H; inv H1; inv H2; inv H3; inv Hv; inv Hv0; try inv Hf; try inv Hf0; clarify;
+        repeat constructor; clarify;
+        rewrite ? H1, ? H2, ? H0, ? H3 in *; clarify.
+        inv Hv1. inv Hv2. unfold transf_globvar in *. clarify. rewrite Hinfo in *.
+        clarify. destruct (transf_vT (gvar_info v2)); inv Hv; inv Hv0.
+        simpl in *. f_equal. f_equal; auto. rewrite Hinit, Hinit0. auto.
+      - inv H; inv H1; inv H2; inv H3; inv Hv; inv Hv0; try inv Hf; try inv Hf0; clarify;
+        repeat constructor; clarify;
+        rewrite ? H1, ? H2, ? H0, ? H3 in *; clarify.
+        intros. apply Hsim.
+        + rewrite <- Hfprog_src. constructor; simpl; auto.
+          unfold globdef_list_linkeq in *. repeat intro.
+          rewrite PTree_unelements_elements. auto.
+        + rewrite <- Hfprog_tgt. constructor; simpl; auto.
+          unfold globdef_list_linkeq in *. repeat intro.
+          rewrite PTree_unelements_elements. auto.
     }
     { eapply globdef_lsim_le; eauto.
       - split; auto. unfold globdef_list_linkeq. rewrite Hle1_src.
@@ -360,32 +338,46 @@ Proof.
   }
   { apply gflink_globdefs in Hdefs_tgt.
     destruct Hdefs_tgt as [i [def1 [def2 [Hdef1 [Hdef2 [H12 H21]]]]]].
-    specialize (H1 i). rewrite Hdef1 in H1.
+    specialize (H1 i). clarify. rewrite Hdef1 in H1.
     destruct ((PTree_unelements defs1_src) ! i) eqn:Hi1_src; [|inv H1].
-    specialize (H2 i). rewrite Hdef2 in H2.
+    specialize (H2 i). clarify. rewrite Hdef2 in H2.
     destruct ((PTree_unelements defs2_src) ! i) eqn:Hi2_src; [|inv H2].
     eapply gtlink_globdefs in Hdefs_src.
     instantiate (1 := i) in Hdefs_src.
     rewrite Hi1_src, Hi2_src in Hdefs_src.
     destruct (defs_src ! i) eqn:Hi_src; [|inv Hdefs_src].
     destruct Hdefs_src as [[]|[]]; subst.
-    { inv H1; inv H2; inv H; inv Hv; try inv Hv0; try inv Hf; try inv Hf0; simplify_decs.
-      { contradict H12. constructor. eapply globfun_linkable_ei; eauto. }
-      { contradict H12. constructor. eapply globfun_linkable_ee; eauto. }
+    { inv H1; inv H2; inv H; inv Hv; try inv Hv0; try inv Hf; try inv Hf0; clarify;
+      rewrite ? H0, ? H1, ? H2 in *; clarify.
+      { contradict H12. constructor. eapply globfun_linkable_ei; eauto.
+        exploit Hsim0; eauto; try reflexivity. intros [_ Hsig1]. inv Hsig1.
+        inv Hsim. exploit transf_efT_sigT; eauto. intro X.
+        clarify. rewrite <- X, Hsig, H0. auto.
+      }
+      { contradict H12. constructor. eapply globfun_linkable_ee; eauto.
+        inv Hsim. inv Hsim0. rewrite H2 in H3. inv H3. auto.
+      }
       { contradict H12. constructor.
         destruct v_src, v_src0. inv Hv1. simpl in *. subst.
         unfold transf_globvar in *. simpl in *.
-        destruct (transf_V gvar_info0); inv Hv; inv Hv2; simpl in *; subst.
+        destruct (transf_vT gvar_info0); inv Hv; inv Hv2; simpl in *; subst.
         constructor; auto.
       }
     }
-    { inv H1; inv H2; inv H; inv Hv; try inv Hv0; try inv Hf; try inv Hf0; simplify_decs.
-      { contradict H21. constructor. eapply globfun_linkable_ei; eauto. }
-      { contradict H21. constructor. eapply globfun_linkable_ee; eauto. }
+    { inv H1; inv H2; inv H; inv Hv; try inv Hv0; try inv Hf; try inv Hf0; clarify;
+      rewrite ? H0, ? H1, ? H2 in *; clarify.
+      { contradict H21. constructor. eapply globfun_linkable_ei; eauto.
+        exploit Hsim; eauto; try reflexivity. intros [_ Hsig1]. inv Hsig1.
+        inv Hsim0. exploit transf_efT_sigT; eauto. intro X.
+        clarify. rewrite <- X, Hsig, H0. auto.
+      }
+      { contradict H21. constructor. eapply globfun_linkable_ee; eauto.
+        inv Hsim. inv Hsim0. rewrite H2 in H3. inv H3. auto.
+      }
       { contradict H21. constructor.
         destruct v_src, v_src0. inv Hv1. simpl in *. subst.
         unfold transf_globvar in *. simpl in *.
-        destruct (transf_V gvar_info); inv Hv; inv Hv2; simpl in *; subst.
+        destruct (transf_vT gvar_info); inv Hv; inv Hv2; simpl in *; subst.
         constructor; auto.
       }
     }
@@ -393,25 +385,25 @@ Proof.
 Qed.
 
 Lemma link_globdef_list_lsim
-      (F_lsim:F_lsimT)
+      (f_lsim:f_lsimT)
       (main:positive)
-      (defs1_src defs2_src:list (positive * globdef fundefT_src V_src))
-      (defs1_tgt defs2_tgt:list (positive * globdef fundefT_tgt V_tgt))
-      defs_src (Hdefs_src: link_globdef_list fundef_src_dec V_src_dec defs1_src defs2_src = Some defs_src)
+      (defs1_src defs2_src:list (positive * globdef fundefT_src vT_src))
+      (defs1_tgt defs2_tgt:list (positive * globdef fundefT_tgt vT_tgt))
+      defs_src (Hdefs_src: link_globdef_list lang_src defs1_src defs2_src = Some defs_src)
       (H1: globdef_list_lsim
-             F_lsim
+             f_lsim
              (mkprogram defs1_src main)
              (mkprogram defs1_tgt main)
              defs1_src defs1_tgt)
       (H2: globdef_list_lsim
-             F_lsim
+             f_lsim
              (mkprogram defs2_src main)
              (mkprogram defs2_tgt main)
              defs2_src defs2_tgt):
   exists defs_tgt,
-    link_globdef_list fundef_tgt_dec V_tgt_dec defs1_tgt defs2_tgt = Some defs_tgt /\
+    link_globdef_list lang_tgt defs1_tgt defs2_tgt = Some defs_tgt /\
     globdef_list_lsim
-      F_lsim
+      f_lsim
       (mkprogram defs_src main)
       (mkprogram defs_tgt main)
       defs_src defs_tgt.
@@ -420,37 +412,37 @@ Proof.
   apply globdef_list_lsim_globdefs_lsim in H2.
   unfold link_globdef_list in Hdefs_src.
   match goal with
-    | [H: context[link_globdefs ?fundef_dec ?V_dec ?defs1 ?defs2] |- _] =>
-      destruct (link_globdefs fundef_dec V_dec defs1 defs2) as [defs|] eqn:Hdefs; inv H
+    | [H: context[link_globdefs ?lang ?defs1 ?defs2] |- _] =>
+      destruct (link_globdefs lang defs1 defs2) as [defs|] eqn:Hdefs; inv H
   end.
   exploit link_globdefs_lsim; eauto. intros [defs_tgt [Hdefs_tgt Hsim]].
-  unfold link_globdef_list. rewrite Hdefs_tgt. eexists. split; eauto.
+  unfold link_globdef_list. clarify. rewrite Hdefs_tgt. eexists. split; eauto.
   apply globdefs_lsim_globdef_list_lsim. auto.
 Qed.
 
 Section DEF.
 
-Variable (F_lsim:F_lsimT).
+Variable (f_lsim:f_lsimT).
 
 Definition F_future_lsim :=
   fun fprog_src fprog_tgt f_src f_tgt =>
     forall (Hfprog: program_weak_lsim fprog_src fprog_tgt),
-    F_lsim fprog_src fprog_tgt f_src f_tgt.
+    f_lsim fprog_src fprog_tgt f_src f_tgt.
 
 Definition program_lsim
-           (prog_src: program fundefT_src V_src)
-           (prog_tgt: program fundefT_tgt V_tgt): Prop :=
+           (prog_src: program fundefT_src vT_src)
+           (prog_tgt: program fundefT_tgt vT_tgt): Prop :=
   globdef_list_lsim F_future_lsim prog_src prog_tgt prog_src.(prog_defs) prog_tgt.(prog_defs) /\
   prog_src.(prog_main) = prog_tgt.(prog_main).
 
 Lemma link_program_lsim
-      (p1_src p2_src:program fundefT_src V_src)
-      (p1_tgt p2_tgt:program fundefT_tgt V_tgt)
-      p_src (Hp_src: link_program fundef_src_dec V_src_dec p1_src p2_src = Some p_src)
+      (p1_src p2_src:program fundefT_src vT_src)
+      (p1_tgt p2_tgt:program fundefT_tgt vT_tgt)
+      p_src (Hp_src: link_program lang_src p1_src p2_src = Some p_src)
       (H1: program_lsim p1_src p1_tgt)
       (H2: program_lsim p2_src p2_tgt):
   exists p_tgt,
-    link_program fundef_tgt_dec V_tgt_dec p1_tgt p2_tgt = Some p_tgt /\
+    link_program lang_tgt p1_tgt p2_tgt = Some p_tgt /\
     program_lsim p_src p_tgt.
 Proof.
   destruct p1_src as [defs1_src main1_src].
@@ -461,7 +453,7 @@ Proof.
   unfold link_program in *. simpl in *. subst.
   destruct ((main1_tgt =? main2_tgt)%positive) eqn:Hmain; [|inv Hp_src].
   apply Pos.eqb_eq in Hmain. subst.
-  destruct (link_globdef_list fundef_src_dec V_src_dec defs1_src defs2_src) as [def_list_src|] eqn:Hdef_list_src; inv Hp_src.
+  destruct (link_globdef_list lang_src defs1_src defs2_src) as [def_list_src|] eqn:Hdef_list_src; inv Hp_src.
   exploit link_globdef_list_lsim; eauto. intros [defs_tgt [Hdefs_tgt Hsim]].
   exists (mkprogram defs_tgt main2_tgt). rewrite Hdefs_tgt. split; auto.
   constructor; auto.
@@ -470,8 +462,8 @@ Qed.
 End DEF.
 
 Lemma program_lsim_le
-      (F_lsim1 F_lsim2:F_lsimT) (HF_lsim: F_lsim1 <4= F_lsim2):
-  (program_lsim F_lsim1) <2= (program_lsim F_lsim2).
+      (f_lsim1 f_lsim2:f_lsimT) (Hf_lsim: f_lsim1 <4= f_lsim2):
+  (program_lsim f_lsim1) <2= (program_lsim f_lsim2).
 Proof.
   intros. destruct PR as [Hdefs Hmain]. split; auto.
   eapply globdef_list_lsim_le; eauto.
@@ -486,11 +478,11 @@ Qed.
 
 Inductive fundef_sig_lsim (f_src:fundefT_src) (f_tgt:fundefT_tgt): Prop :=
 | fundef_sig_lsim_intro
-    (Hsig: fundef_sig_src f_src = fundef_sig_tgt f_tgt)
+    (Hsig: sig_lsim (fd_sig_src f_src) (fd_sig_tgt f_tgt))
 .
 
 Inductive fundef_weak_lsim
-          (ge_src:Genv.t fundefT_src V_src) (ge_tgt:Genv.t fundefT_tgt V_tgt)
+          (ge_src:Genv.t fundefT_src vT_src) (ge_tgt:Genv.t fundefT_tgt vT_tgt)
           (f_src:fundefT_src) (f_tgt:fundefT_tgt): Prop :=
 | fundef_weak_lsim_intro
     (Hsig: fundef_sig_lsim f_src f_tgt)
@@ -501,40 +493,43 @@ Inductive fundef_weak_lsim
 
 Section INITIALIZE.
 
-Variable (fprog_src: program fundefT_src V_src).
-Variable (fprog_tgt: program fundefT_tgt V_tgt).
-Variable (F_lsim:F_lsimT).
-Variable (Hfprog: program_lsim_aux F_lsim fprog_src fprog_tgt).
+Variable (fprog_src: program fundefT_src vT_src).
+Variable (fprog_tgt: program fundefT_tgt vT_tgt).
+Variable (f_lsim:f_lsimT).
+Variable (Hfprog: program_lsim_aux f_lsim fprog_src fprog_tgt).
 
 Inductive match_fundef (f_src:fundefT_src) (f_tgt:fundefT_tgt): Prop :=
 | match_fundef_intro
     (Hsig: fundef_sig_lsim f_src f_tgt)
-    (Hsim: globfun_lsim F_lsim fprog_src fprog_tgt f_src f_tgt)
+    (Hsim: globfun_lsim f_lsim fprog_src fprog_tgt f_src f_tgt)
 .
 
 Let ge_src := Genv.globalenv fprog_src.
 Let ge_tgt := Genv.globalenv fprog_tgt.
 
 Lemma program_lsim_match_program:
-  match_program match_fundef V_lsim nil fprog_src.(prog_main) fprog_src fprog_tgt.
+  match_program match_fundef v_lsim nil fprog_src.(prog_main) fprog_src fprog_tgt.
 Proof.
   unfold match_program. destruct Hfprog as [Hfdefs Hmain].
   split; eauto. exists fprog_tgt.(prog_defs). split; [|rewrite app_nil_r; auto].
-  revert Hfdefs. generalize (prog_defs fprog_src) as l1, (prog_defs fprog_tgt) as l2.
+  revert Hfdefs. clarify. generalize (prog_defs fprog_src) as l1, (prog_defs fprog_tgt) as l2.
   induction l1; intros l2 Hsim; inv Hsim; constructor; auto.
   destruct a, b1, H1. simpl in *. subst.
   inv H0.
-  - repeat constructor; auto.
-    inv Hf; unfold fundef_sig_src, fundef_sig_tgt; rewrite Hsrc, Htgt; auto.
-    exploit (Hsim fprog_src fprog_tgt); eauto; try reflexivity.
-    intros [_ ?]. auto.
+  - inv Hf. clarify.
+    destruct (Fundef_dec (fundefT lang_src) f_src) eqn:Hsrc,
+             (Fundef_dec (fundefT lang_tgt) f_tgt) eqn:Htgt; try (inv Hsim; fail).
+    + exploit Hsim; try reflexivity. intros [_ ?].
+      repeat constructor; clarify; rewrite Hsrc, Htgt; auto.
+    + repeat constructor; clarify; rewrite Hsrc, Htgt; auto.
+      apply transf_efT_sigT. auto.
   - destruct v_src, v_tgt. inv Hv. unfold transf_globvar in Hv0. simpl in *.
-    destruct (transf_V gvar_info) eqn:Hgvar_info; inv Hv0. constructor; auto.
+    destruct (transf_vT gvar_info) eqn:Hgvar_info; inv Hv0. constructor; auto.
 Qed.
 Local Hint Resolve program_lsim_match_program.
 
 Lemma globalenvs_match:
-  Genv.match_genvs match_fundef V_lsim nil (Genv.globalenv fprog_src) (Genv.globalenv fprog_tgt).
+  Genv.match_genvs match_fundef v_lsim nil (Genv.globalenv fprog_src) (Genv.globalenv fprog_tgt).
 Proof. eapply Genv.globalenvs_match; eauto. Qed.
 Local Hint Resolve globalenvs_match.
 
@@ -558,7 +553,7 @@ Lemma varinfo_preserved:
     match Genv.find_var_info (Genv.globalenv fprog_tgt) b, Genv.find_var_info (Genv.globalenv fprog_src) b with
       | None, None => True
       | Some v_tgt, Some v_src =>
-        transf_globvar transf_V v_src = OK v_tgt
+        transf_globvar transf_vT v_src = OK v_tgt
       | _, _ => False
     end.
 Proof.
@@ -587,7 +582,7 @@ Lemma funct_ptr_translated':
   forall (b : block) (f : fundefT_src),
   Genv.find_funct_ptr (Genv.globalenv fprog_src) b = Some f ->
   exists tf : fundefT_tgt,
-  Genv.find_funct_ptr (Genv.globalenv fprog_tgt) b = Some tf /\ globfun_lsim F_lsim fprog_src fprog_tgt f tf.
+  Genv.find_funct_ptr (Genv.globalenv fprog_tgt) b = Some tf /\ globfun_lsim f_lsim fprog_src fprog_tgt f tf.
 Proof.
   intros. exploit Genv.find_funct_ptr_match; eauto. intros [tf [Htf Hsim]].
   exists tf. split; auto. inv Hsim. auto.
@@ -605,7 +600,7 @@ Qed.
 
 Lemma sig_preserved:
   forall f tf (Hsim: fundef_sig_lsim f tf),
-    fundef_sig_src f = fundef_sig_tgt tf.
+    sig_lsim (fd_sig_src f) (fd_sig_tgt tf).
 Proof.
   intros. inv Hsim. auto.
 Qed.
