backend/Tailcallproof_linker.v
@@ -35,25 +35,19 @@ Hypothesis TRANSF: transf_program prog = tprog.
 Section FUTURE.
 
 Variable (fprog ftprog:program).
-Hypothesis (Hfsim: program_weak_lsim
-                     fundef_dec fn_sig fundef_dec fn_sig transf_V
-                     fprog ftprog).
+Hypothesis (Hfsim: @program_weak_lsim Language_RTL Language_RTL id (@Errors.OK _) transf_V
+                                      fprog ftprog).
 
-Hypothesis (Hfprog: program_linkeq fundef_dec prog fprog).
-Hypothesis (Hftprog: program_linkeq fundef_dec tprog ftprog).
+Hypothesis (Hfprog: program_linkeq Language_RTL prog fprog).
+Hypothesis (Hftprog: program_linkeq Language_RTL tprog ftprog).
 
 Let globfun_weak_lsim :=
-  globfun_lsim fundef_dec fn_sig fundef_dec fn_sig (fun _ _ _ _ => True) fprog ftprog.
+  @globfun_lsim Language_RTL Language_RTL id (@Errors.OK _)
+                (fun _ _ _ _ => True)
+                fprog ftprog.
 
 Let ge := Genv.globalenv fprog.
 Let tge := Genv.globalenv ftprog.
-
-Let rm := romem_for_program prog.
-
-Lemma rm_frm: PTree_le rm (romem_for_program fprog).
-Proof.
-  apply program_linkeq_romem_le. auto.
-Qed.
 
 Inductive match_stackframes: list stackframe -> list stackframe -> Prop :=
   | match_stackframes_nil:
@@ -101,7 +95,7 @@ Inductive match_call: state -> state -> Prop :=
   | match_states_call:
       forall s f args m s' f' args' m',
       match_stackframes s s' ->
-      fundef_weak_lsim fundef_dec fn_sig fundef_dec fn_sig ge tge f f' ->
+      fundef_weak_lsim Language_RTL Language_RTL id ge tge f f' ->
       Val.lessdef_list args args' ->
       Mem.extends m m' ->
       match_call (Callstate s f args m)
@@ -298,10 +292,10 @@ Proof.
   exploit funct_ptr_translated; eauto. intros [tf [A B]].
   exists (Callstate nil tf nil m0); split.
   econstructor; eauto.
-  eapply program_lsim_init_mem_match; eauto.
+  eapply (@program_lsim_init_mem_match Language_RTL Language_RTL); try apply transf_efT_sigT; eauto.
   replace (prog_main ftprog) with (prog_main fprog).
   erewrite symbols_preserved; eauto.
-  destruct Hfsim as [_ Hmain]. unfold fundef in *. rewrite <- Hmain. auto.
+  destruct Hfsim as [_ Hmain]. unfold fundef in *. simpl in *. rewrite <- Hmain. auto.
   rewrite <- H3. eapply sig_preserved; eauto.
   constructor. constructor. auto. auto. apply Mem.extends_refl.
 Qed.
@@ -372,12 +366,11 @@ Qed.
 Section STATE_LSIM.
 
 Variable (fprog ftprog:program).
-Hypothesis (Hfsim: program_weak_lsim
-                     fundef_dec fn_sig fundef_dec fn_sig transf_V
-                     fprog ftprog).
+Hypothesis (Hfsim: @program_weak_lsim Language_RTL Language_RTL id (@Errors.OK _) transf_V
+                                      fprog ftprog).
 
-Hypothesis (Hfprog: program_linkeq fundef_dec prog fprog).
-Hypothesis (Hftprog: program_linkeq fundef_dec tprog ftprog).
+Hypothesis (Hfprog: program_linkeq Language_RTL prog fprog).
+Hypothesis (Hftprog: program_linkeq Language_RTL tprog ftprog).
 
 Lemma match_states_state_lsim es es' eF F s1 s1'
       (MS: match_states_ext fprog ftprog s1 s1'):
@@ -461,10 +454,9 @@ Qed.
 End STATE_LSIM.
 
 Lemma Tailcall_program_lsim:
-  program_lsim
-    fundef_dec fn_sig fundef_dec fn_sig transf_V
-    (function_lsim mrelT_ops)
-    prog tprog.
+  @program_lsim Language_RTL Language_RTL id (@Errors.OK _) transf_V
+                (function_lsim mrelT_ops)
+                prog tprog.
 Proof.
   generalize transf_function_lsim.
   destruct prog as [defs main]. simpl in *.
@@ -475,17 +467,16 @@ Proof.
   induction defs; simpl; intros fdefs Hlsim; simpl; [constructor|].
   destruct a. destruct g.
   - constructor; simpl in *; try apply IHdefs; auto.
-    split; auto. constructor.
+    split; auto. apply (@globdef_lsim_fun Language_RTL Language_RTL).
     destruct f; simpl in *.
-    + eapply globfun_lsim_i; eauto; unfold fundef_dec, common_fundef_dec; eauto.
+    + eapply globfun_lsim_intro; eauto; simpl; auto.
       split; auto. repeat intro.
       apply Hlsim; auto.
       unfold transf_function. destruct (zeq (fn_stacksize f) 0 && Compopts.eliminate_tailcalls tt); simpl; auto.
-    + eapply globfun_lsim_e; eauto;
-      unfold fundef_dec, common_fundef_dec; eauto.
+    + eapply globfun_lsim_intro; eauto; simpl; auto.
   - constructor; simpl in *; try apply IHdefs; auto.
-    split; auto. repeat constructor.
-    unfold transf_globvar. simpl. destruct v; auto.
+    split; auto. apply (@globdef_lsim_var Language_RTL Language_RTL).
+    repeat constructor. destruct v; auto.
 Qed.
 
 End PRESERVATION.
