common/LinkerProp.v
@@ -10,16 +10,34 @@ Set Implicit Arguments.
 
 Section LINKER_PROP.
 
-Variable (fundefT F V:Type).
-Variable (fundef_dec: fundef_decT fundefT F).
-Variable (V_dec: forall (v1 v2:V), {v1 = v2} + {v1 <> v2}).
+Variable (lang:Language).
+  
+Let sigT := lang.(sigT).
+Let fT := lang.(fT).
+Let efT := lang.(efT).
+Let fundefT := lang.(fundefT).
+Let vT := lang.(vT).
 
-Lemma gflink_globdefs defs1 defs2 (Hlink: link_globdefs fundef_dec V_dec defs1 defs2 = None):
+Let f_sig := fT.(F_sig).
+Let ef_sig := efT.(EF_sig).
+Let ef_dec := efT.(EF_dec).
+Let fundef_dec := fundefT.(Fundef_dec).
+Let v_dec := vT.(V_dec).
+
+Ltac clarify :=
+  repeat
+    (try match goal with
+           | [H1: fundef_dec ?f = _, H2: fundef_dec ?f = _ |- _] =>
+             rewrite H1 in H2; inv H2
+         end;
+     auto).
+
+Lemma gflink_globdefs defs1 defs2 (Hlink: link_globdefs lang defs1 defs2 = None):
   exists var def1 def2,
     PTree.get var defs1 = Some def1 /\
     PTree.get var defs2 = Some def2 /\
-    ~ globdef_linkable fundef_dec def1 def2 /\
-    ~ globdef_linkable fundef_dec def2 def1.
+    ~ globdef_linkable lang def1 def2 /\
+    ~ globdef_linkable lang def2 def1.
 Proof.
   unfold link_globdefs in Hlink.
   match goal with
@@ -30,17 +48,17 @@ Proof.
   destruct Hlinkable as [i [x [Hx1 Hx2]]].
   destruct x; inv Hx2. rewrite PTree.gcombine in Hx1; auto.
   destruct (defs1 ! i) eqn:Hi1, (defs2 ! i) eqn:Hi2; inv Hx1.
-  destruct (globdef_linkable_dec fundef_dec V_dec g g0); inv H0.
-  destruct (globdef_linkable_dec fundef_dec V_dec g0 g); inv H1.
+  destruct (globdef_linkable_dec lang g g0); inv H0.
+  destruct (globdef_linkable_dec lang g0 g); inv H1.
   repeat eexists; eauto.
 Qed.
 
-Lemma gtlink_globdefs defs1 defs2 defs (Hlink: link_globdefs fundef_dec V_dec defs1 defs2 = Some defs):
+Lemma gtlink_globdefs defs1 defs2 defs (Hlink: link_globdefs lang defs1 defs2 = Some defs):
   forall var,
     match PTree.get var defs1, PTree.get var defs2, PTree.get var defs with
       | Some g1, Some g2, Some g =>
-        (globdef_linkable fundef_dec g1 g2 /\ g2 = g) \/
-        (globdef_linkable fundef_dec g2 g1 /\ g1 = g)
+        (globdef_linkable lang g1 g2 /\ g2 = g) \/
+        (globdef_linkable lang g2 g1 /\ g1 = g)
       | Some g1, None, Some g => g1 = g
       | None, Some g2, Some g => g2 = g
       | None, None, None => True
@@ -54,16 +72,16 @@ Proof.
   end.
   rewrite PTree_goption_map, PTree.gcombine; auto.
   destruct (defs1 ! i) eqn:Hi1, (defs2 ! i) eqn:Hi2; auto.
-  destruct (globdef_linkable_dec fundef_dec V_dec g g0).
+  destruct (globdef_linkable_dec lang g g0).
   { left. split; auto. }
-  destruct (globdef_linkable_dec fundef_dec V_dec g0 g).
+  destruct (globdef_linkable_dec lang g0 g).
   { right. split; auto. }
   eapply PTree_Properties.for_all_correct in Hlinkable; eauto.
   { instantiate (1 := None) in Hlinkable. inv Hlinkable. }
   instantiate (1 := i). rewrite PTree.gcombine; auto.
   rewrite Hi1, Hi2.
-  destruct (globdef_linkable_dec fundef_dec V_dec g g0); try (contradict n; auto; fail).
-  destruct (globdef_linkable_dec fundef_dec V_dec g0 g); try (contradict n0; auto; fail).
+  destruct (globdef_linkable_dec lang g g0); try (contradict n; auto; fail).
+  destruct (globdef_linkable_dec lang g0 g); try (contradict n0; auto; fail).
   auto.
 Qed.
 
